Finite set enhancements
- Unicode syntax
- new fSIGMA constant
- registration in TypeBase (for induction and cases)
- finite_setSyntax library

src/pred_set/src/more_theories/finite_setSyntax.sig
@@ -1,0 +1,22 @@
+signature finite_setSyntax =
+sig
+
+  include Abbrev
+  val fset_ty : hol_type
+  val mk_fset_ty : hol_type -> hol_type
+  val empty_tm : term
+  val in_tm : term
+  val insert_tm : term
+  val inter_tm : term
+  val union_tm : term
+
+  val mk_empty : hol_type -> term
+  val mk_in : term * term -> term
+  val mk_insert : term * term -> term
+  val mk_union : term * term -> term
+  val mk_inter : term * term -> term
+  val mk_set : term list * hol_type -> term
+  val mk_set1 : term list -> term
+
+
+end
