src/pred_set/src/more_theories/finite_setSyntax.sml
@@ -1,0 +1,33 @@
+structure finite_setSyntax :> finite_setSyntax =
+struct
+
+open HolKernel boolLib
+open finite_setTheory
+
+val ERR = mk_HOL_ERR "finite_setSyntax"
+
+
+val s2 = HolKernel.syntax_fns2 "finite_set"
+
+fun mk_fset_ty elty = mk_thy_type{Args = [elty], Thy = "finite_set", Tyop = "fset"}
+
+val fset_ty = mk_fset_ty alpha
+fun mk_empty ty = mk_thy_const{Name = "fEMPTY", Thy = "finite_set",
+                               Ty = mk_fset_ty ty}
+
+val empty_tm = mk_empty alpha
+
+val (in_tm, mk_in, dest_in, is_in) = s2 "fIN"
+val (insert_tm, mk_insert, dest_insert, is_insert) = s2 "fINSERT"
+val (union_tm, mk_union, dest_union, is_union) = s2 "fUNION"
+val (inter_tm, mk_inter, dest_inter, is_inter) = s2 "fINTER"
+
+fun mk_set(l, ty) =
+    List.foldr mk_insert (mk_empty ty) l
+fun mk_set1 l =
+    case l of
+        [] => raise ERR "mk_set1" "Empty list"
+      | h::_ => mk_set(l, type_of h)
+
+
+end (* struct *)
